add ffdhe_precomp_p

code/ffdhe/Hacl.FFDHE.fst
@@ -18,6 +18,11 @@ let ke (a:S.ffdhe_alg) =
 
 private
 [@CInline]
+let ffdhe_precomp_p (a:S.ffdhe_alg) : DH.ffdhe_precomp_p_st t_limbs a (DH.ffdhe_len a) (ke a) =
+  DH.ffdhe_precomp_p a (DH.ffdhe_len a) (ke a)
+
+private
+[@CInline]
 let ffdhe_check_pk (a:S.ffdhe_alg) : DH.ffdhe_check_pk_st t_limbs a (DH.ffdhe_len a) =
   DH.ffdhe_check_pk #t_limbs a (DH.ffdhe_len a)
 
@@ -29,15 +34,36 @@ let ffdhe_compute_exp (a:S.ffdhe_alg) : DH.ffdhe_compute_exp_st t_limbs a (DH.ff
 
 let ffdhe_len (a:S.ffdhe_alg) : DH.size_pos = DH.ffdhe_len a
 
+
+val new_ffdhe_precomp_p: a:S.ffdhe_alg ->
+  DH.new_ffdhe_precomp_p_st t_limbs a (ffdhe_len a) (ke a)
+let new_ffdhe_precomp_p a =
+  DH.new_ffdhe_precomp_p a (DH.ffdhe_len a) (ke a) (ffdhe_precomp_p a)
+
+
+val ffdhe_secret_to_public_precomp: a:S.ffdhe_alg ->
+  DH.ffdhe_secret_to_public_precomp_st t_limbs a (DH.ffdhe_len a) (ke a)
+let ffdhe_secret_to_public_precomp a p_r2_n sk pk =
+  let len = DH.ffdhe_len a in
+  DH.ffdhe_secret_to_public_precomp a len (ke a) (ffdhe_compute_exp a) p_r2_n sk pk
+
+
 val ffdhe_secret_to_public: a:S.ffdhe_alg ->
   DH.ffdhe_secret_to_public_st t_limbs a (DH.ffdhe_len a) (ke a)
 let ffdhe_secret_to_public a sk pk =
   let len = DH.ffdhe_len a in
-  DH.ffdhe_secret_to_public a len (ke a) (ffdhe_compute_exp a) sk pk
+  DH.ffdhe_secret_to_public a len (ke a) (ffdhe_secret_to_public_precomp a) (ffdhe_precomp_p a) sk pk
+
+
+val ffdhe_shared_secret_precomp: a:S.ffdhe_alg ->
+  DH.ffdhe_shared_secret_precomp_st t_limbs a (DH.ffdhe_len a) (ke a)
+let ffdhe_shared_secret_precomp a p_r2_n sk pk ss =
+  let len = DH.ffdhe_len a in
+  DH.ffdhe_shared_secret_precomp a len (ke a) (ffdhe_check_pk a) (ffdhe_compute_exp a) p_r2_n sk pk ss
 
 
 val ffdhe_shared_secret: a:S.ffdhe_alg ->
   DH.ffdhe_shared_secret_st t_limbs a (DH.ffdhe_len a) (ke a)
 let ffdhe_shared_secret a sk pk ss =
   let len = DH.ffdhe_len a in
-  DH.ffdhe_shared_secret a len (ke a) (ffdhe_check_pk a) (ffdhe_compute_exp a) sk pk ss
+  DH.ffdhe_shared_secret a len (ke a) (ffdhe_shared_secret_precomp a) (ffdhe_precomp_p a) sk pk ss
