code/ffdhe/Hacl.FFDHE4096.fsti
@@ -25,6 +25,13 @@ let len = normalize_term (DH.ffdhe_len a_ffdhe) //=512
 inline_for_extraction noextract
 val ke_4096 : BE.exp t_limbs
 
+
+val new_ffdhe_precomp_p: DH.new_ffdhe_precomp_p_st t_limbs a_ffdhe len ke_4096
+
+val ffdhe_secret_to_public_precomp: DH.ffdhe_secret_to_public_precomp_st t_limbs a_ffdhe len ke_4096
+
 val ffdhe_secret_to_public: DH.ffdhe_secret_to_public_st t_limbs a_ffdhe len ke_4096
+
+val ffdhe_shared_secret_precomp: DH.ffdhe_shared_secret_precomp_st t_limbs a_ffdhe len ke_4096
 
 val ffdhe_shared_secret: DH.ffdhe_shared_secret_st t_limbs a_ffdhe len ke_4096
